DiagonaLean/Rice/Reductions.lean
@@ -6,26 +6,21 @@ Authors: Kshitij Salunke
 
 import DiagonaLean.Synthetic.Definitions
 import DiagonaLean.Synthetic.Undecidability
+import DiagonaLean.Synthetic.ReductionChain
 import DiagonaLean.Rice.Basic
 
 open DiagonaLean.Synthetic.Notation DiagonaLean.Synthetic.Definitions DiagonaLean.Rice
+open DiagonaLean.Synthetic.ReductionChain
 
 variable {X Y : Type*}
 
-def meow (f : X → Y) (p : X → Prop) (q : Y → Prop) : Prop := reduction f p q
-
-theorem undecidablity_of_reduction {X Y : Type*} {P1 : X → Prop} {P2 : Y → Prop}
+/-- If `P1` reduces to `P2` and `P1` is undecidable, then `P2` is undecidable. -/
+theorem undecidability_of_reduction {X Y : Type*} {P1 : X → Prop} {P2 : Y → Prop}
   (h_red : P1 ⪯ₘ P2) : ¬ SDecidable P1 → ¬ SDecidable P2 := by
   intro hs1 hs2
-  have h : SDecidable P1 := by
-    rcases h_red with ⟨f, hf⟩
-    rcases hs2 with ⟨g, hg⟩
-    use g ∘ f
-    intro x
-    rw [hf x]
-    exact hg (f x)
-  contradiction
+  exact hs1 (dec_red h_red hs2)
 
+/-- If `P1` reduces to `P2` and `P1` is not semi-decidable, then `P2` is not semi-decidable. -/
 theorem un_semi_decidability_of_reduction {X Y : Type*} {P1 : X → Prop} {P2 : Y → Prop}
   (h_red : P1 ⪯ₘ P2): ¬ semi_decidable P1 → ¬ semi_decidable P2 := by
   intro hs1 hs2
@@ -38,16 +33,7 @@ theorem un_semi_decidability_of_reduction {X Y : Type*} {P1 : X → Prop} {P2 : 
     exact hg (f x)
   contradiction
 
-theorem decidability_of_reduction {X Y : Type*} {P1 : X → Prop} {P2 : Y → Prop}
-  (h_red : P1 ⪯ₘ P2) : SDecidable P2 → SDecidable P1 := by
-  intro hs2
-  rcases h_red with ⟨f, hf⟩
-  rcases hs2 with ⟨g, hg⟩
-  use g ∘ f
-  intro x
-  rw [hf x]
-  exact hg (f x)
-
+/-- If `P1` reduces to `P2` and `P2` is semi-decidable, then `P1` is semi-decidable. -/
 theorem semi_decidability_of_reduction {X Y : Type*} {P1 : X → Prop} {P2 : Y → Prop}
   (h_red : P1 ⪯ₘ P2) : semi_decidable P2 → semi_decidable P1 := by
   intro hs2
